DynamoDbEncryption/dafny/DynamoDbEncryption/test/FilterExpr.dfy
@@ -401,6 +401,32 @@ module TestDynamoDBFilterExpr {
     expect_equal(newItems, []);
   }
 
+  method {:test} TestFromExample() {
+    var names : DDB.ExpressionAttributeNameMap := map [
+      "#p" := "PK1",
+      "#sk1" := "SK1",
+      "#dur" := "Duration"
+    ];
+    var values : DDB.ExpressionAttributeValueMap := map [
+      ":e" := DS("EE-able@gmail.com"),
+      ":date1" := DS("MS-2022-07-02"),
+      ":date2" := DS("MS-2022-07-08"),
+      ":dur" := DS("0")
+    ];
+
+    var context := ExprContext (
+      expr := Some("#p = :e AND #sk1 BETWEEN :date1 AND :date2"),
+      values:= Some(values),
+      names := Some(names)
+    );
+
+    var version := GetLotsaBeacons();
+    var src := GetLiteralSource([1,2,3,4,5], version);
+    var bv :- expect ConvertVersionWithSource(FullTableConfig, version, src);
+    var newContext :- expect Beaconize(bv, context, DontUseKeyId);
+
+  }
+
   method {:test} TestFilterAttrOps() {
     var names : DDB.ExpressionAttributeNameMap := map [
       "#fecha" := "Date"
@@ -493,11 +519,46 @@ module TestDynamoDBFilterExpr {
     var bv :- expect ConvertVersionWithSource(FullTableConfig, version, src);
     var newItems := FilterResults(bv, [SimpleItem], None, Some("NameTitle between :val3 and :val4"), None, Some(values));
     expect newItems.Failure?;
-    expect newItems.error == E("To use BETWEEN with a compound beacon, the part after any common prefix must be nonsensitive.");
+    print "\n", newItems.error, "\n";
+    expect newItems.error == E("To use BETWEEN with a compound beacon, the part after any common prefix must be nonsensitive, or just a prefix : BETWEEN T_ATitle AND T_MyTitle");
   }
 
-  /*
-    Successes :
-      compound beacon on virtual field
-  */
+  method {:test} TestComparisons() {
+
+    var values : DDB.ExpressionAttributeValueMap := map [
+      ":val1" := DS("N_"),
+      ":val2" := DS("N_MyName"),
+      ":val3" := DS("N_MyName.T_"),
+      ":val4" := DS("N_MyName.T_Title"),
+      ":val5" := DS("T_"),
+      ":val6" := DS("N_MyName.N_")
+    ];
+
+    var version := GetLotsaBeacons();
+    var src := GetLiteralSource([1,2,3,4,5], version);
+    var bv :- expect ConvertVersionWithSource(FullTableConfig, version, src);
+
+    var newItems := FilterResults(bv, [SimpleItem], None, Some("NameTitle between :val1 and :val5"), None, Some(values));
+    expect newItems.Success?;
+    newItems := FilterResults(bv, [SimpleItem], None, Some("NameTitle between :val3 and :val6"), None, Some(values));
+    expect newItems.Success?;
+    newItems := FilterResults(bv, [SimpleItem], None, Some("NameTitle between :val2 and :val3"), None, Some(values));
+    expect newItems.Success?;
+
+    newItems := FilterResults(bv, [SimpleItem], None, Some("NameTitle between :val1 and :val2"), None, Some(values));
+    expect newItems.Failure?;
+    newItems := FilterResults(bv, [SimpleItem], None, Some("NameTitle between :val1 and :val4"), None, Some(values));
+    expect newItems.Failure?;
+
+    newItems := FilterResults(bv, [SimpleItem], None, Some("NameTitle < :val1"), None, Some(values));
+    expect newItems.Success?;
+    newItems := FilterResults(bv, [SimpleItem], None, Some("NameTitle = :val1"), None, Some(values));
+    expect newItems.Success?;
+    newItems := FilterResults(bv, [SimpleItem], None, Some("NameTitle < :val2"), None, Some(values));
+    expect newItems.Success?;
+    newItems := FilterResults(bv, [SimpleItem], None, Some("NameTitle = :val2"), None, Some(values));
+    expect newItems.Failure?;
+
+  }
+
 }
